theories/lang/notation.v
@@ -11,6 +11,11 @@ Coercion Var : string >-> expr.
 Coercion BNamed : string >-> binder.
 Notation "<>" := BAnon : lrust_binder_scope.
 
+Notation "[ x ]" := (@cons expr x%E (@nil expr)) : expr_scope.
+Notation "[ x1 ; x2 ; .. ; xn ]" :=
+  (@cons expr x1%E (@cons expr x2%E
+        (..(@cons expr xn%E (@nil expr))..))) : expr_scope.
+
 (* No scope for the values, does not conflict and scope is often not inferred
 properly. *)
 Notation "# l" := (LitV l%Z%V) (at level 8, format "# l").
