theories/typing/tests/get_x.v
@@ -1,0 +1,39 @@
+From lrust.lifetime Require Import definitions.
+From lrust.lang Require Import new_delete.
+From lrust.typing Require Import programs product product_split own uniq_bor
+                    shr_bor int function lft_contexts uninit cont.
+
+Section get_x.
+  Context `{typeG Σ}.
+
+  Definition get_x :=
+    (funrec: "get_x" ["p"] → "ret" :=
+       let: "p'" := !"p" in
+       letalloc: "r" := "p'" +ₗ #0 in
+       delete [ #1; "p"] ;; "ret" ["r":expr])%E.
+
+  Lemma get_x_type :
+    typed_instruction_ty [] [] [] get_x
+        (fn (λ α, [☀α])%EL (λ α, [# own 1 (&uniq{α}Π[int; int])])
+            (λ α, own 1 (&shr{α} int))).
+  Proof.
+    apply type_fn; try apply _. intros α get_x ret args. inv_vec args=>p args.
+    inv_vec args. simpl_subst.
+
+    eapply type_let'.
+    { apply _. }
+    { by apply (type_deref (&uniq{α}Π [int; int])), read_own_move. }
+    { solve_typing. }
+    intros p'. simpl_subst.
+
+    eapply (type_letalloc_1 (&shr{α}int)); (try solve_typing)=>r. simpl_subst.
+
+    eapply type_let'.
+    { apply _. }
+    { eapply (type_delete (uninit 1) 1); solve_typing. }
+    { solve_typing. }
+    move=> /= _.
+
+    eapply type_jump with (args := [r]); solve_typing.
+  Qed.
+End get_x.
